\onecolumn
\section{Hyperspherical Form of Adaptive Contrastive Loss}
We have the initial formulation of the adaptive contrastive loss
\begin{equation}
\mathcal{L}_{\text{AdaptiveCE}} = -\sum_{i=1}^{B} \epsilon^p_i \cdot \text{sim}(\mathbf{t}^1_i, \mathbf{t}^2_i) + \sum_{j=1, k=1, j \neq k}^{B} \epsilon_{j,k}^n \cdot \text{sim}(\mathbf{t}_j^{1}, \mathbf{t}_k^{2})
\end{equation}
We first substitute $\epsilon_i^p = [o^p - \text{sim}(\mathbf{t}^1_i, \mathbf{t}^2_i)]_+$ and $\epsilon_{j,k}^n = [\text{sim}(\mathbf{t}^1_j, \mathbf{t}^2_k) - o^n]_+$ into the above equation,
\begin{align}
& \mathcal{L}_{\text{AdaptiveCE}} = \sum_{i=1}^{B} \text{sim}(\mathbf{t}^1_i, \mathbf{t}^2_i)^2 - o^p \cdot \text{sim}(\mathbf{t}^1_i, \mathbf{t}^2_i)  + \sum_{j=1, k=1, j \neq k}^{B} \text{sim}(\mathbf{t}^1_i, \mathbf{t}^2_i)^2 - o^n \cdot \text{sim}(\mathbf{t}^1_j, \mathbf{t}^2_k) \\
& = \sum_{i=1}^{B} \left(\text{sim}(\mathbf{t}^1_i, \mathbf{t}^2_i) - \frac{o^p}{2}\right)^2 + \sum_{j=1, k=1, j \neq k}^{B} \left(\text{sim}(\mathbf{t}^1_j, \mathbf{t}^2_k) - \frac{o^n}{2}\right)^2 - C 
\end{align}
where $C =  \left(\frac{o^p}{2}\right)^2 + \left(\frac{o^n}{2}\right)^2$. Now we obtain the spherical form of our contrastive loss.